Fix the definition of core_data for the extended machine simulation. There's still some work to be done to show that the generalized lex order on this type is well founded.  In particular, we may need to require that the total number of cores be bounded.

veric/extension_proof.v
@@ -641,7 +641,15 @@ Inductive compilability_invariant: Type := CompilableExtension: forall
     Forall2 Val.has_type vals2 (sig_args sig) -> 
     exists cd, exists s2, 
       make_initial_core (esem target) ge v2 vals2 = Some s2 /\
-      match_states cd j s1 m1 s2 m2),
+      match_states cd j s1 m1 s2 m2)
+
+  (safely_halted_diagram: forall cd j c1 m1 c2 m2 ge v1,
+    match_states cd j c1 m1 c2 m2 -> 
+    safely_halted (esem source) ge c1 = Some v1 -> 
+    exists v2,
+      val_inject j v1 v2 /\
+      safely_halted (esem target) ge c2 = Some v2 /\ 
+      Mem.inject j m1 m2),
   compilability_invariant.
 
 Variables (esig_compilable: compilability_invariant)
@@ -867,40 +875,12 @@ Qed.
 Next Obligation. 
 inv esig_compilable.
 eapply make_initial_core_diagram; eauto.
-(*rename H0 into INIT.
-rename H1 into INJ.
-rename H2 into VALINJ.
-rename H3 into TYPE.
-inv core_compat1.
-destruct (Extension.active_csem E1 c1) as [CS CORES].
-destruct (Extension.active_proj_core E1 c1) as [_c1 PROJ1].
-destruct (make_init1 ge c1 v1 vals1 (ACTIVE E1 c1) CS CORES INIT)
- as [_c1' [INIT' PROJ1']].
-rewrite PROJ1' in PROJ1.
-inv PROJ1.
-unfold cores in CORES.
-inv CORES.
-generalize (core_initial core_simulation v1 v2 sig H vals1 _c1 m1 j vals2 m2 INIT');
- intro MATCH.
-spec MATCH; auto.
-spec MATCH; auto.
-spec MATCH; auto.
-destruct MATCH  as [cd [_c2 [? ?]]].
-exists cd.
-clear make_init2.
-inv core_compat2.
-specialize (make_init2 ge _c2 v2 vals2 O target).
-spec make_init2; auto.
-spec make_init2; auto.
-destruct make_init2 as [c2 [INIT2 MATCH2]].
-exists c2.
-split; auto.*)
 Qed.
 
 Next Obligation. 
-rename H into MATCH; hnf in MATCH.
-destruct MATCH as [ACT [RUN MATCH_CORES]].
-Admitted. (*TODO*)
+inv esig_compilable.
+eapply safely_halted_diagram; eauto.
+Qed.
 
 Next Obligation. 
 rename H into MATCH.
@@ -1047,8 +1027,71 @@ Module ExtensionSimulations2. Section ExtensionSimulations2.
 
  Definition core_datas := forall i:nat, core_data (core_simulations i).
 
- Definition core_ords (cd1 cd2: core_datas) := forall (i:nat), 
-   core_ord (core_simulations i) (cd1 i) (cd2 i).
+ Definition core_datas_upd
+   i (cdi': core_data (core_simulations i)) (cd: core_datas): core_datas :=
+   fun j: nat => 
+     match eq_nat_dec i j as pf in sumbool _ _ return core_data (core_simulations j) with
+     | left pf => match pf with
+                  | eq_refl => cdi'
+                  end
+     | right pf => cd j
+     end.
+
+ Lemma core_datas_upd_same i cdi' cd: (core_datas_upd i cdi' cd) i = cdi'.
+ Proof.
+ unfold core_datas_upd.
+ destruct (eq_nat_dec i i).
+ rewrite (UIP_refl _ _ e); auto.
+ elimtype False; auto.
+ Qed.
+
+ Lemma core_datas_upd_other i j cdi' cd: i<>j -> (core_datas_upd i cdi' cd) j = cd j.
+ Proof.
+ unfold core_datas_upd.
+ destruct (eq_nat_dec i j).
+ intros; elimtype False; auto.
+ auto.
+ Qed.
+
+ Variable max_cores: nat. (*I don't think it's possible to build a well-founded order
+                             on infinite products; so we just bound the number of cores.*)
+
+ Definition core_ords_aux (i: nat) (cd1 cd2: core_datas): Prop := 
+   core_ord (core_simulations i) (cd1 i) (cd2 i) /\
+   (forall j, (j < i)%nat -> cd1 j=cd2 j).
+
+ Lemma core_ords_aux0: forall cd1 cd2,
+   core_ords_aux O cd1 cd2 <-> core_ord (core_simulations O) (cd1 O) (cd2 O). 
+ Proof.
+ intros cd1 cd2.
+ unfold core_ords_aux.
+ split.
+ intros [H1 H2]; auto.
+ intros H1.
+ split; auto.
+ intros j CONTRA.
+ elimtype False; omega.
+ Qed.
+
+ Definition core_ords cd1 cd2 := 
+   exists i, (i < max_cores)%nat /\ core_ords_aux i cd1 cd2.
+
+ Lemma core_ords_wf: well_founded core_ords.
+ Proof.
+ unfold core_ords.
+ induction max_cores.
+ constructor.
+ intros b [i [H1 H2]].
+ elimtype False; omega.
+ constructor.
+ intros b [i [H1 [H2 H3]]].
+ destruct (IHn a) as [H4].
+ specialize (H4 b).
+ generalize (core_ord_wf (core_simulations i)).
+ intros H5.
+ destruct (H5 (a i)) as [H6].
+ specialize (H6 (b i) H2).
+ Admitted. (*TODO*)
 
  Notation PROJ_CORE := (Extension.proj_core).
  Infix "\o" := (Extension.zmult) (at level 66, left associativity). 
@@ -1179,7 +1222,15 @@ Module ExtensionSimulations2. Section ExtensionSimulations2.
     Forall2 Val.has_type vals2 (sig_args sig) -> 
     exists cd, exists s2, 
       make_initial_core esemT ge v2 vals2 = Some s2 /\
-      match_states cd j s1 m1 s2 m2),
+      match_states cd j s1 m1 s2 m2)
+
+  (safely_halted_diagram: forall cd j c1 m1 c2 m2 ge v1,
+    match_states cd j c1 m1 c2 m2 -> 
+    safely_halted esemS ge c1 = Some v1 -> 
+    exists v2,
+      val_inject j v1 v2 /\
+      safely_halted esemT ge c2 = Some v2 /\ 
+      Mem.inject j m1 m2),
   compilability_invariant.
 
  Variables 
@@ -1190,7 +1241,7 @@ Program Definition extended_simulation:
   Forward_simulation_inject dS dT esemS esemT ge ge entry_points :=
       Build_Forward_simulation_inject 
       core_datas match_states core_ords _ _ _ _ _ _.
-Next Obligation. unfold core_ords, core_datas. Admitted. (*TODO*)
+Next Obligation. apply core_ords_wf. Qed.
 Next Obligation. 
 rename H0 into MATCH.
 generalize MATCH as MATCH'; intro.
@@ -1241,7 +1292,9 @@ spec CSTEPN; auto.
 spec CSTEPN; auto. 
 spec CSTEPN; auto.
 destruct CSTEPN as [st2' [ESEM2 [ACT2' PROJ2']]].
-exists st2'; exists m2'; exists cd; exists j'.
+exists st2'; exists m2'.
+exists (core_datas_upd (ACTIVE E_S st1) cd' cd).
+exists j'.
 split3; auto.
 split; auto.
  (*Subgoal: match_states*)
@@ -1268,9 +1321,7 @@ split; auto.
   rewrite PROJ1' in _PROJ1'.
   inv _PROJ1'.
   split; auto.
-  assert (Hxx: cd' = cd i).
-   admit.
-  rewrite <-Hxx; auto.
+  solve[rewrite core_datas_upd_same; auto].
 
   (*ACTIVE E_S st1 <> i*)
   intros NEQ _.
@@ -1310,7 +1361,7 @@ split; auto.
   exists _d; split; auto.
   inv esig_compilable.
   specialize (match_others i cd j j' st1 cd' (cd i) c1 m1 c1' m1' st2 c2 m2 c2' m2' _c _d (S n)).
-  solve[spec match_others; auto; auto].
+  solve[rewrite core_datas_upd_other; auto].
   solve[left; exists n; auto].
 
 (*corestep_star case*)
@@ -1323,7 +1374,9 @@ spec CSTEPN; auto.
 spec CSTEPN; auto. 
 spec CSTEPN; auto.
 destruct CSTEPN as [st2' [ESEM2 [ACT2' PROJ2']]].
-exists st2'; exists m2'; exists cd; exists j'.
+exists st2'; exists m2'. 
+exists (core_datas_upd (ACTIVE E_S st1) cd' cd).
+exists j'.
 split3; auto.
 split; auto.
  (*Subgoal: match_states*)
@@ -1349,9 +1402,7 @@ split; auto.
   rewrite PROJ1' in _PROJ1'.
   inv _PROJ1'.
   split; auto.
-  assert (Hxx: cd' = cd i).
-   admit.
-  rewrite <-Hxx; auto.
+  solve[rewrite core_datas_upd_same; auto].
 
   (*ACTIVE E_S st1 <> i*)
   intros NEQ _.
@@ -1391,8 +1442,9 @@ split; auto.
   exists _d; split; auto.
   inv esig_compilable.
   specialize (match_others i cd j j' st1 cd' (cd i) c1 m1 c1' m1' st2 c2 m2 c2' m2' _c _d n).
-  solve[spec match_others; auto; auto].
-  right. split. exists n. auto. admit. (*fix core_ord*)
+  solve[rewrite core_datas_upd_other; auto].
+  right. split. exists n. auto. 
+   admit. (*should follow from ORD and definition of generalized lex_prod*)
 
 (*runnable = false*)
 intros RUN1.
@@ -1436,9 +1488,8 @@ inv esig_compilable; eapply make_initial_core_diagram; eauto.
 Qed.
 
 Next Obligation. 
-rename H into MATCH; hnf in MATCH.
-destruct MATCH as [ACT [RUN MATCH_CORES]].
-Admitted. (*TODO*)
+inv esig_compilable; eapply safely_halted_diagram; eauto.
+Qed.
 
 Next Obligation. 
 rename H into MATCH.
@@ -1480,7 +1531,8 @@ destruct (core_after_external (core_simulations (ACTIVE E_S st1))
                 (cd (ACTIVE E_S st1)) j j' c1 c2 m1 e 
                 vals1 ret1 m1' m2 m2' ret2 ef_sig)
  as [cd' [c1' [c2' [AFTER1 [AFTER2 MATCH12']]]]]; auto.
-exists cd. (*FIXME*)
+
+exists (core_datas_upd (ACTIVE E_S st1) cd' cd).
 assert (exists st1', after_external esemS (Some ret1) st1 = Some st1' /\
          PROJ_CORE E_S (ACTIVE E_S st1) st1' = Some c1') as [st1' [? PROJ1']].
  inv core_compat1.
@@ -1521,9 +1573,7 @@ intros EQ _; subst.
 exists c2'; split; auto.
 rewrite _PROJ1' in PROJ1'.
 inv PROJ1'; auto.
-assert (cd' = cd i) as <-.
- admit.
-auto.
+solve[rewrite core_datas_upd_same; auto].
 
 (*ACTIVE E_S st1 <> i*)
 intros NEQ _.
